src/ConcreteEvidence.v
@@ -13,13 +13,14 @@ Notation BS := nat (only parsing).
 (** * Concrete Evidence *)
 Inductive EvidenceC: Set :=
 | mtc: EvidenceC
-| uuc: ASP_ID -> (* Plc -> *) BS -> EvidenceC -> EvidenceC
-| ggc: (*Plc ->*) BS -> EvidenceC -> EvidenceC
-| hhc: (*Plc ->*) BS -> EvidenceC -> EvidenceC (* TODO: remove Ev param *)
-| nnc: (*Plc ->*) N_ID -> BS -> EvidenceC -> EvidenceC
+| uuc: ASP_ID -> BS -> EvidenceC -> EvidenceC
+| ggc: BS -> EvidenceC -> EvidenceC
+| hhc: BS -> EvidenceC -> EvidenceC (* TODO: remove Ev param *)
+| nnc: N_ID -> BS -> EvidenceC -> EvidenceC
 | ssc: EvidenceC -> EvidenceC -> EvidenceC
 | ppc: EvidenceC -> EvidenceC -> EvidenceC.
 
+(*
 (** * Concrete Evidence *)
 Inductive AnnoEvidenceC: Set :=
 | amtc: AnnoEvidenceC
@@ -29,7 +30,7 @@ Inductive AnnoEvidenceC: Set :=
 | annc: (*nat ->*) (*Plc ->*) N_ID -> BS -> AnnoEvidenceC -> AnnoEvidenceC
 | assc: AnnoEvidenceC -> AnnoEvidenceC -> AnnoEvidenceC
 | appc: AnnoEvidenceC -> AnnoEvidenceC -> AnnoEvidenceC.
-
+*)
 
 
 (*
@@ -49,9 +50,9 @@ Fixpoint et_fun (p:Plc) (ec:EvidenceC) : Evidence :=
 
 Inductive Ev_Shape: EvidenceC -> Evidence -> Prop :=
 | mtt: Ev_Shape mtc mt
-| uut: forall id p bs e et,
+| uut: forall id args p bs e et,
     Ev_Shape e et ->
-    Ev_Shape (uuc id bs e) (uu id p et)
+    Ev_Shape (uuc id bs e) (uu id args p et)
 | ggt: forall p bs e et,
     Ev_Shape e et ->
     Ev_Shape (ggc bs e) (gg p et)
