src/Appraisal3.v
@@ -1,0 +1,1453 @@
+Require Import GenStMonad MonadVM MonadAM ConcreteEvidence.
+Require Import StAM VM_IO_Axioms Maps VmSemantics Event_system Term_system.
+
+Require Import Coq.Arith.Peano_dec.
+
+Require Import StructTactics.
+
+Require Import Coq.Program.Tactics Coq.Program.Equality.
+
+Require Import List.
+Import ListNotations.
+
+Set Nested Proofs Allowed.
+
+
+Inductive evidenceEvent: Ev -> Prop :=
+| uev: forall n p i args, evidenceEvent (umeas n p i args)
+(*| sev: forall n p, evidenceEvent (sign n p)
+| hev: forall n p, evidenceEvent (hash n p)*) .
+
+(*
+Definition measEvent (t:AnnoTerm) (p:Plc) (ev:Ev) : Prop :=
+  let es := ev_sys t p in
+  ev_in ev es /\ evidenceEvent ev.
+ *)
+
+Definition measEvent (t:AnnoTerm) (p:Plc) (ev:Ev) : Prop :=
+  events t p ev /\ evidenceEvent ev.
+
+Check bound_to.
+
+Inductive appEvent : Ev -> AM_St -> Ev -> Prop :=
+| aeu : forall p q i i' n m args nmap nid amap,
+    bound_to amap (p,i) i' ->
+    appEvent (umeas n p i args) (mkAM_St nmap nid amap) (umeas m q i' (args ++ [n])).
+
+Definition am_get_app_asp (p:Plc) (i:ASP_ID) : AM ASP_ID :=
+  m <- gets st_aspmap ;;
+  let maybeId := map_get m (p,i) in
+  match maybeId with
+  | Some i' => ret i'
+  | None => failm
+  end.
+
+Fixpoint gen_appraisal_comp (e:EvidenceC) (et:Evidence) : AM (VM unit) :=
+  match e with
+  | mtc =>
+    match et with
+    | mt => ret (ret tt)
+    | _ => failm
+    end   
+  | uuc i bs e' =>
+    match et with 
+    | uu i_t args_t p e'_t =>
+      app_id <- am_get_app_asp p i_t ;;
+      let c1 :=
+          e <- invokeUSM 0 app_id p (args_t ++ [bs]) ;;  (* TODO: is bogus event id ok here? *)
+          put_ev e in
+      c2 <- gen_appraisal_comp e' e'_t ;;
+      ret (c1 ;; c2)
+    | _ => failm
+    end
+  | ggc bs e' =>
+    match et with
+    | gg p e'_t =>
+      ret (ret tt)
+    | _ => failm
+    end
+  | hhc bs e' =>
+    match et with
+    | hh p e'_t =>
+      ret (ret tt)
+    | _ => failm
+    end
+  | nnc nid bs e' =>
+    match et with
+    | nn nid_t e'_t =>
+      ret (ret tt)
+    | _ => failm
+    end
+  | ssc e1 e2 =>
+    match et with
+    | ss e1_t e2_t => 
+      c1 <- gen_appraisal_comp e1 e1_t ;;
+          c2 <- gen_appraisal_comp e2 e2_t ;;
+          ret (c1 ;; c2)
+    | _ => failm
+    end
+  | ppc e1 e2 =>
+    match et with
+    | ss e1_t e2_t => 
+      c1 <- gen_appraisal_comp e1 e1_t ;;
+          c2 <- gen_appraisal_comp e2 e2_t ;;
+          ret (c1 ;; c2)
+    | _ => failm
+    end
+  end.
+
+Check build_comp.
+Check runSt.
+Check run_vm.
+Check eval.
+
+(*
+Definition run_vm_fresh (t:AnnoTerm) :=
+  run_vm t empty_vmst.
+Check run_vm_fresh.
+
+
+Definition run_vm_fresh_t (t:Term) :=
+  run_vm (annotated t) empty_vmst.
+Check run_vm_fresh_t.
+*)
+
+Definition build_app_comp (t: AnnoTerm) (p:Plc) (st:vm_st) : AM (VM unit) :=
+  let vm_res_st := run_vm t st in
+  let evc := st_ev vm_res_st in
+  let evt := eval (unanno t) p mt in
+  app_comp <- gen_appraisal_comp evc evt ;;
+  ret (app_comp).
+
+Definition build_app_comp_t (t:Term) (p:Plc) (st:vm_st) : AM (VM unit) :=
+  build_app_comp (annotated t) p st.
+
+Definition exec_app_comp (t: AnnoTerm) (p:Plc) (st:vm_st) : AM vm_st :=
+  app_comp <- build_app_comp t p st ;;
+  let app_res := runSt empty_vmst app_comp in
+  ret ((snd (app_res))).
+
+Definition exec_app_comp_t (t: Term) (p:Plc) (p':nat) (st:vm_st) : AM vm_st :=
+  exec_app_comp (snd (anno t p')) p st.
+
+Definition run_app_comp_ev (t: AnnoTerm) (p:Plc) (st:vm_st) : AM EvidenceC :=
+  app_st <- exec_app_comp t p st ;;
+  ret (st_ev app_st).
+
+Definition run_app_comp_ev_t (t: Term) (p:Plc) (st:vm_st) : AM EvidenceC :=
+  run_app_comp_ev (annotated t) p st.
+  
+
+(*
+Definition at1 := (asp (ASPC 11 [])).
+Definition at2 := (asp (ASPC 22 [])).
+Definition aterm := bseq (NONE,NONE) at1 at2.
+
+
+Definition aterm_ev_comp := run_app_comp_ev_t aterm 0.
+
+Definition ast :=
+  mkAM_St [] 0 [((0,11),34); ((0,22),45)].
+
+Definition aterm_res : ((option EvidenceC) * AM_St) := runSt ast aterm_ev_comp.
+Compute aterm_res.
+
+Definition aterm_st : AM vm_st := exec_app_comp_t aterm 0 0.
+Compute (runSt ast aterm_st).
+
+Definition aet := eval aterm 0 mt.
+Compute aet.
+
+Definition evc_st := (run_vm_fresh_t aterm).
+Compute evc_st.
+Definition evc := st_ev evc_st.
+Compute evc.
+*)
+
+Definition fromOpt{A:Type} (o:option A) (a:A) : A :=
+  match o with
+  | Some t => t
+  | None => a
+  end.
+
+Definition allMapped (t:AnnoTerm) (p:Plc) (st: AM_St) : Prop :=
+  forall aspmap n q i l ,
+    measEvent t p (umeas n q i l) -> (* TODO: generalize once measEvent is richer *)
+    aspmap = st_aspmap st ->
+    exists j,
+      bound_to aspmap (q,i) j.
+
+Lemma atgentrace : forall t p e n v1 v a b am_nonceMap am_nonceId st_aspmap ev,
+    gen_appraisal_comp
+      (st_ev (snd (build_comp (annotated t) empty_vmst))) (eval t p e)
+      {| am_nonceMap := am_nonceMap; am_nonceId := am_nonceId; st_aspmap := st_aspmap |} = (Some v1, a) ->
+    gen_appraisal_comp
+      (st_ev (snd (build_comp (annotated (att n t)) empty_vmst))) (eval (att n t) p e)
+      {| am_nonceMap := am_nonceMap; am_nonceId := am_nonceId; st_aspmap := st_aspmap |} = (Some v, b) ->
+    In ev (st_trace (snd (v1 empty_vmst))) ->
+    In ev (st_trace (snd (v empty_vmst))).
+Proof.
+Admitted.
+
+Lemma fifi : forall t p e n v a b am_nonceMap am_nonceId st_aspmap,
+    gen_appraisal_comp
+      (st_ev (snd (build_comp (annotated t) empty_vmst))) (eval t p e)
+      {| am_nonceMap := am_nonceMap; am_nonceId := am_nonceId; st_aspmap := st_aspmap |} = (Some v, a) ->
+    gen_appraisal_comp
+      (st_ev (snd (build_comp (annotated (att n t)) empty_vmst))) (eval t n mt)
+      {| am_nonceMap := am_nonceMap; am_nonceId := am_nonceId; st_aspmap := st_aspmap |} = (None, b) ->
+    False.
+Proof.
+Admitted.
+
+
+
+Lemma measEventAt' : forall t n p q ev,
+    measEvent (snd (anno (att n t) q)) p ev ->
+    measEvent (snd (anno t (S q))) n ev.
+Proof.
+
+  induction t; intros.
+  - inv H.
+    invc H1.
+    destruct a;
+      try (inv H; inv H1; solve_by_inversion).
+    +
+      simpl in *.
+      invc H0.
+      invc H6.
+      invc H.
+      invc H0.
+      simpl.
+      econstructor.
+      eauto.
+      eauto.
+  -
+    simpl in *.
+    repeat break_let.
+    simpl in *.
+    repeat find_inversion.
+    simpl in *.
+    invc H.
+    invc H1.
+    repeat find_inversion.
+    invc H0.
+    invc H5.
+    econstructor.
+    +
+    econstructor.
+    assumption.
+    +
+      econstructor.
+  - simpl in *.
+    repeat break_let.
+    simpl in *.
+    repeat find_inversion.
+    simpl in *.
+    invc H.
+    invc H1.
+    repeat find_inversion.
+    invc H0.
+    invc H5.
+    econstructor.
+    econstructor.
+    eassumption.
+    econstructor.
+    econstructor.
+    apply evtslseqr.
+    assumption.
+    econstructor.
+  - simpl in *.
+    repeat break_let.
+    simpl in *.
+    repeat find_inversion.
+    simpl in *.
+    invc H.
+    invc H1.
+    repeat find_inversion.
+    invc H0.
+    invc H5.
+    econstructor.
+    econstructor.
+    eassumption.
+    econstructor.
+    econstructor.
+    apply evtsbseqr.
+    assumption.
+    econstructor.
+  - simpl in *.
+    repeat break_let.
+    simpl in *.
+    repeat find_inversion.
+    simpl in *.
+    invc H.
+    invc H1.
+    repeat find_inversion.
+    invc H0.
+    invc H5.
+    econstructor.
+    econstructor.
+    eassumption.
+    econstructor.
+    econstructor.
+    apply evtsbparr.
+    assumption.
+    econstructor.
+Defined.
+
+(*
+Lemma measEventAt : forall t n p ev,
+    measEvent (annotated (att n t)) p ev ->
+    measEvent (annotated t) n ev.
+Proof.
+  intros.
+  eapply measEventAt'.
+  eapply measEventAt'; eauto.
+Defined.
+*)
+
+
+Lemma announ' : forall t p,
+    unanno (snd (anno t p)) = t.
+Proof.
+  induction t; intros; unfold annotated; simpl.
+  -
+    auto.
+  - repeat break_let. simpl.
+    edestruct IHt with (p:=(S p)).
+    rewrite Heqp0.
+    simpl.
+    reflexivity.
+  - repeat break_let.
+    simpl.
+    edestruct IHt1 with (p:=p).
+    rewrite Heqp0. simpl.
+    edestruct IHt2 with (p:=n).
+    rewrite Heqp1. simpl. eauto.
+  - repeat break_let.
+    simpl.
+    edestruct IHt1 with (p:=S p).
+    rewrite Heqp0. simpl.
+    edestruct IHt2 with (p:=n).
+    rewrite Heqp1. simpl. eauto.
+  - repeat break_let.
+    simpl.
+    edestruct IHt1 with (p:=S p).
+    rewrite Heqp0. simpl.
+    edestruct IHt2 with (p:=n).
+    rewrite Heqp1. simpl. eauto.
+Defined.
+
+Lemma announ : forall t,
+    unanno (annotated t) = t.
+Proof.
+  intros.
+  eapply announ'; eauto.
+Defined.
+
+Lemma allMappedAt : forall r n a p st,
+    allMapped (aatt r n a) p st ->
+    allMapped a n st.
+Proof.
+  intros.
+  unfold allMapped.
+  intros; subst.
+  invc H0.
+  unfold allMapped in H.
+  assert (measEvent a n (umeas n0 q i l)).
+  econstructor; eauto.
+
+  edestruct H.
+  econstructor.
+  econstructor.
+  eassumption.
+  econstructor.
+  reflexivity.
+  eauto.
+Defined.
+
+Check exec_app_comp_t.
+Check runSt.
+
+Require Import MonadVMFacts.
+
+
+Lemma app_some' :
+  
+
+Lemma app_some : forall t p p' vm_st vm_st' app_comp app_comp_res a_st,
+    build_comp (snd (anno t p')) vm_st = (Some tt, vm_st') ->
+    allMapped (snd (anno t p')) p a_st ->
+    app_comp = exec_app_comp_t t p p' vm_st ->
+    app_comp_res = runSt a_st app_comp ->
+    exists st, (fst app_comp_res = (Some st)).
+Proof.
+  induction t; intros; subst.
+  -
+
+    destruct a.
+    + unfold exec_app_comp_t.
+      unfold exec_app_comp.
+      monad_unfold.
+      monad_unfold.
+      repeat find_inversion.
+      unfold runSt.
+      repeat break_match.
+      simpl.
+      eexists. eauto.
+      unfold build_app_comp in *.
+      cbn in *.
+      vmsts.
+      simpl in *.
+      monad_unfold.
+      repeat break_match; try solve_by_inversion.
+      repeat find_inversion.
+      monad_unfold.
+      repeat break_let.
+      simpl in *.
+      unfold runSt.
+      cbn.
+      assert (st_ev = mtc).
+      admit.
+      subst.
+      inv Heqp1.
+    +
+      vmsts.
+      simpl in *.
+      monad_unfold.
+      repeat find_inversion.
+      unfold runSt.
+      cbn.
+      unfold exec_app_comp_t.
+      unfold exec_app_comp.
+      monad_unfold.
+      unfold build_app_comp.
+      monad_unfold.
+      monad_unfold.
+      unfold allMapped in H0.
+      break_match.
+      repeat break_match.
+      repeat break_let.
+      repeat find_inversion.
+      unfold runSt.
+      repeat break_let.
+      eexists. simpl.
+      eauto.
+      repeat find_inversion.
+      solve_by_inversion.
+      solve_by_inversion.
+      solve_by_inversion.
+      solve_by_inversion.
+      solve_by_inversion.
+      solve_by_inversion.
+      solve_by_inversion.
+      repeat find_inversion.
+      repeat find_inversion.
+      monad_unfold.
+      cbn in *.
+      repeat break_let.
+      repeat find_inversion.
+      repeat break_match; try solve_by_inversion.
+      edestruct H0.
+      econstructor. econstructor. reflexivity. econstructor.
+      reflexivity.
+      inv H.
+      repeat find_inversion.
+      subst.
+      rewrite H1 in *.
+      repeat find_inversion.
+      destruct a_st.
+      simpl in *.
+      monad_unfold.
+      repeat find_inversion.
+      simpl in *
+      
+  +
+  break_match.
+  break_match.
+  admit.
+  unfold build_app_comp in *.
+  unfold run_vm in *.
+  unfold execSt in *.
+  unfold build_comp in *.
+  unfold bind in *.
+  unfold do_prim in *.
+  unfold copyEv in *.
+  unfold add_tracem in *.
+  unfold modify in *.
+  repeat break_let.
+  simpl in *.
+  destruct o0; try solve_by_inversion.
+  simpl in *.
+  destruct o1; try solve_by_inversion.
+  simpl in *.
+  repeat find_inversion.
+  destruct vm_st.
+  simpl in *.
+  repeat find_inversion.
+  
+  monad_unfold.
+  break_match.
+  
+  repeat break_match; try solve_by_inversion; simpl in *.
+  simpl in *.
+  vmsts.
+  repeat find_inversion.
+  solve_by_inversion.
+  simpl in *.
+  repeat find_inversion.
+  repeat find_inversion.
+  + monad_unfold.
+    simpl in *.
+    cbn.
+    break_match.
+    repeat break_let.
+    simpl in *.
+    subst.
+    cbv.
+    repeat find_inversion.
+    repeat break_let.
+    destruct o.
+    ++
+      repeat break_let.
+      repeat find_inversion.
+      eexists. eauto.
+    ++ repeat find_inversion.
+       unfold build_app_comp in *.
+       monad_unfold.
+       repeat break_match; try solve_by_inversion.
+       repeat find_inversion.
+       unfold allMapped in *.
+       edestruct H0 with (aspmap:=st_aspmap a_st).
+       econstructor.
+       
+       
+      
+    eexists.
+    reflexivity.
+  + cbn.
+    unfold build_app_comp.
+    monad_unfold.
+    monad_unfold.
+    unfold allMapped in *.
+    edestruct H0.
+    econstructor.
+    econstructor.
+    simpl.
+    reflexivity.
+    econstructor.
+    reflexivity.
+    unfold am_get_app_asp.
+    monad_unfold.
+    inv H1.
+    rewrite H2.
+    simpl.
+    eexists. reflexivity.
+  +
+    cbn.
+    eexists.
+    reflexivity.
+  + cbn.
+    eexists.
+    reflexivity.
+  -
+    unfold exec_app_comp_t.
+    unfold exec_app_comp.
+    monad_unfold.
+    unfold runSt.
+    repeat break_let.
+    unfold snd in *.
+    assert (exists vvss, (build_comp a empty_vmst) = (Some tt, vvss)).
+    {
+      admit.
+    }
+    destruct_conjs.
+    
+    cbn in *.
+    repeat break_let.
+    monad_unfold.
+    unfold get_store_at in *.
+    monad_unfold.
+    repeat break_let.
+    dohtac.
+    repeat find_inversion.
+    break_match.
+    +
+      repeat break_let.
+      simpl.
+      eauto.
+
+      (*
+      subst.
+      unfold build_app_comp in *.
+      monad_unfold.
+      simpl in *.
+      cbn in *.
+      unfold run_vm_fresh in *.
+      cbn in *.
+      unfold run_vm in *.
+      monad_unfold.
+      monad_unfold.
+      repeat break_let.
+      unfold get_store_at in *.
+      monad_unfold.
+      repeat break_let.
+      dohtac.
+      repeat find_inversion.
+      simpl in *.
+      destruct o; try solve_by_inversion.
+      repeat find_inversion.
+      edestruct IHt.
+      rewrite Heqp0.
+      eassumption.
+      rewrite Heqp0.
+      eapply allMappedAt; eauto.
+      reflexivity.
+      reflexivity.
+      unfold exec_app_comp_t in *.
+      unfold exec_app_comp in *.
+      monad_unfold.
+      rewrite Heqp0 in *.
+      simpl in *.
+      unfold runSt in *.
+      Print gen_appraisal_comp.
+      Print build_app_comp.
+      unfold build_app_comp in *.
+      monad_unfold.
+      assert (
+          (toRemote (unanno a) n mtc) =
+          (st_ev (run_vm_fresh a))).
+      {
+        admit.
+      }
+      rewrite <- H3 in *.
+      rewrite Heqp2 in *.
+      repeat find_inversion.
+      simpl in *.
+      rewrite Heqp8 in *.
+      simpl in *.
+      eexists.
+      reflexivity. *)
+    +
+      unfold build_app_comp in *.
+      monad_unfold.
+      unfold run_vm_fresh in *.
+      cbn in *.
+      unfold run_vm in *.
+      monad_unfold.
+      monad_unfold.
+      repeat break_let.
+      unfold get_store_at in *.
+      monad_unfold.
+      dohtac.
+      repeat find_inversion.
+      simpl in *.
+      destruct o0; try solve_by_inversion.
+      repeat find_inversion.
+      edestruct IHt.
+      rewrite Heqp0.
+      eassumption.
+      rewrite Heqp0.
+      eapply allMappedAt; eauto.
+      reflexivity.
+      reflexivity.
+      unfold exec_app_comp_t in *.
+      unfold exec_app_comp in *.
+      monad_unfold.
+      unfold runSt in *.
+      rewrite Heqp0 in *.
+      simpl in *.
+      unfold build_app_comp in *.
+      monad_unfold.
+
+      assert ((toRemote (unanno a) n mtc) =
+              (st_ev (run_vm_fresh a))).
+      {
+        admit.
+      }
+      rewrite <- H3 in *.
+      rewrite Heqp2 in *.
+      simpl in *.
+      congruence.
+  -
+    destruct ((snd (anno (lseq t1 t2) p'))) eqn:hi;
+      try (inv hi;
+           repeat break_let;
+           simpl in *;
+           solve_by_inversion).
+
+
+
+
+    unfold empty_vmst in *.
+    vmsts.
+    edestruct alseq_decomp; eauto.
+    destruct_conjs.
+    repeat break_let.
+
+    unfold exec_app_comp_t.
+    unfold exec_app_comp.
+    monad_unfold.
+    unfold runSt.
+    repeat break_let.
+    simpl in *.
+
+    destruct o; try solve_by_inversion.
+    repeat find_inversion.
+    rewrite Heqp6 in *.
+    repeat find_inversion.
+
+    destruct o1.
+    + admit.
+    +
+      
+
+    assert ((allMapped (alseq (p', n0) a1 a2) p a_st) -> False).
+    admit.
+    tauto.
+
+
+
+
+
+
+
+
+
+
+
+
+
+
+
+
+    
+    repeat find_inversion.
+    unfold build_app_comp in *.
+    monad_unfold.
+    unfold run_vm_fresh in *.
+    unfold run_vm in *.
+    monad_unfold.
+    simpl in *.
+    monad_unfold.
+    unfold empty_vmst in *.
+    rewrite Heqp2 in *.
+    monad_unfold.
+    simpl in *.
+    repeat break_let.
+    simpl in *.
+    simpl in *.
+    repeat break_let.
+    simpl in *.
+    rewrite Heqp6 in *.
+    repeat find_inversion.
+    repeat break_let.
+
+    repeat break_match;
+      try solve_by_inversion.
+    +
+      repeat find_inversion.
+      destruct v0.
+      simpl.
+      eexists. eauto.
+    +
+      repeat find_inversion.
+      destruct v.
+      simpl in *.
+      destruct o0.
+      dunit.
+      repeat find_inversion.
+      
+      eapply fals.
+      rewrite Heqp6. reflexivity.
+      
+      
+
+    unfold gen_appraisal_comp in *
+                                 
+
+
+
+
+    
+    rewrite <- Heqp6 in *.
+
+    assert ( (let (_, y) := anno t2 p' in y) =  (let (_, y) := anno t2 p' in y)
+    
+      
+      
+      
+      unfold 
+      
+      
+      unfold gen_appraisal_comp in *
+      eapply IHt.
+      unfold gen_appraisal_comp in *
+      
+    
+    
+    
+    
+      
+    
+    
+  
+
+Lemma app_correct :
+  forall t app_comp app_comp_res app_comp_st tr_app_comp ev p p' a_st st',
+
+    build_comp (snd (anno t p')) empty_vmst = (Some tt, st') ->
+    app_comp = exec_app_comp_t t p p'  (* AM vm_st *) ->
+    app_comp_res = runSt a_st app_comp (* ((option vm_st) * AM_St) *)  -> 
+    app_comp_st = fromOpt (fst app_comp_res) empty_vmst (* vm_st *)  ->
+    tr_app_comp = st_trace app_comp_st ->
+                      
+    measEvent (snd (anno t p')) p ev ->
+    allMapped (snd (anno t p')) p a_st ->
+    exists ev', In ev' tr_app_comp /\ appEvent ev a_st ev'.
+Proof.
+  induction t; intros; subst.
+  -
+    destruct a;
+      try (invc H4;
+           invc H1;
+           solve_by_inversion).
+    +
+      inv H4.
+      inv H1.
+      inv H0.
+      simpl in *.
+      repeat find_inversion.
+         
+      simpl in *.
+      monad_unfold.
+      unfold allMapped in *.
+      edestruct H5.
+      eassumption.
+      reflexivity.
+      unfold am_get_app_asp.
+      inv H2.
+      unfold exec_app_comp_t.
+      unfold exec_app_comp.
+      unfold build_app_comp.
+      monad_unfold.
+      monad_unfold.
+      unfold runSt.
+      unfold am_get_app_asp.
+      monad_unfold.
+      repeat break_let.
+      rewrite H3 in *.
+      simpl in *.
+      repeat find_inversion.
+      simpl in *.
+      Print appEvent.
+      eexists.
+      split.
+      eauto.
+      destruct a.
+      Print appEvent.
+      econstructor.
+      eauto.
+  -
+    inv H4.
+    inv H1.
+    cbn in *.
+    repeat break_let.
+    unfold snd in *.
+    assert ((build_comp a empty_vmst) = (Some tt, st')).
+    {
+      admit.
+    }
+    
+    simpl in *.
+    inv H0.
+
+    assert (allMapped a n a_st).
+    eapply allMappedAt; eauto.
+        
+    unfold allMapped in H5.
+    edestruct H5.
+    eassumption.
+    reflexivity.
+    inv H6.
+    
+    edestruct IHt.
+    rewrite Heqp1.
+    eassumption.
+    reflexivity.
+    reflexivity.
+    reflexivity.
+    reflexivity.
+    eapply measEventAt'.
+    assert ((aatt (p',S n1) n a) = (snd (anno (att n t) p'))) as HH.
+    {
+      cbn. repeat break_let.
+      simpl.
+      congruence.
+    }
+    rewrite <- HH. clear HH.
+    eassumption.
+    rewrite Heqp1.
+    simpl.
+    eassumption.
+
+    exists x0.
+    unfold exec_app_comp_t in *.
+    unfold exec_app_comp in *.
+    monad_unfold.
+    rewrite Heqp1 in *.
+    simpl in *.
+    unfold runSt in *.
+    simpl in *.
+    repeat break_let.
+    unfold get_store_at in *.
+    monad_unfold.
+    repeat break_let.
+    dohtac.
+    repeat find_inversion.
+    repeat break_match; try solve_by_inversion.
+    +
+      repeat find_inversion.
+      simpl in *.
+      repeat find_inversion.
+      cbn in *.
+      unfold build_app_comp in *.
+      monad_unfold.
+      cbn in *.
+
+      unfold run_vm_fresh in *.
+      unfold run_vm in Heqp7.
+      unfold execSt in Heqp7.
+      cbn in Heqp7.
+      repeat break_let.
+      repeat find_inversion.
+      monad_unfold.
+      repeat find_inversion.
+      unfold get_store_at in *.
+      monad_unfold.
+      repeat break_let.
+      dohtac.
+      repeat find_inversion.
+      simpl in *.
+      assert ((st_ev (run_vm a empty_vmst)) = (toRemote (unanno a) n mtc)).
+      {
+        admit. (* TODO: make this an axiom? *)
+      }
+      rewrite H in *.
+      subst.
+      rewrite Heqp6 in *.
+      repeat find_inversion.
+      repeat break_match; try solve_by_inversion.
+      repeat find_inversion.
+      eassumption.
+    + simpl in *.
+      tauto.
+    + simpl in *.
+      repeat find_inversion.
+      unfold build_app_comp in *.
+      monad_unfold.
+      unfold run_vm_fresh in *.
+      cbn in *.
+      unfold run_vm in Heqp7.
+      monad_unfold.
+      monad_unfold.
+      repeat break_let.
+      repeat find_inversion.
+      simpl in *.
+      unfold get_store_at in *. monad_unfold. repeat break_let.
+      dohtac.
+      repeat find_inversion.
+      simpl in *.
+
+       assert ((st_ev (run_vm a empty_vmst)) = (toRemote (unanno a) n mtc)).
+      {
+        admit. (* TODO: make this an axiom? *)
+      }
+      rewrite H in *.
+      rewrite Heqp9 in *.
+      repeat find_inversion.
+      repeat break_match; solve_by_inversion.
+  -
+    invc H4.
+    invc H1.
+    invc H0; repeat break_let; simpl in *; try solve_by_inversion; invc H1.
+    +
+    unfold exec_app_comp_t.
+    unfold exec_app_comp.
+    monad_unfold.
+    simpl in *.
+    repeat break_let.
+    unfold snd in *.
+    (*build_comp (alseq (p', n3) a1 a2) empty_vmst = (Some tt, st')*)
+    Print build_app_comp.
+    unfold runSt.
+    unfold build_app_comp.
+    monad_unfold.
+    unfold run_vm_fresh.
+    unfold run_vm.
+    unfold execSt.
+    cbn.
+    rewrite H.
+    simpl in *.
+    unfold runSt.
+    simpl in *.
+    repeat break_match; try solve_by_inversion; repeat find_inversion.
+    ++
+      simpl in *.
+      unfold build_app_comp in *.
+      monad_unfold.
+      repeat find_inversion.
+      unfold run_vm_fresh in *.
+      unfold run_vm in *.
+      monad_unfold.
+      monad_unfold.
+      simpl in *.
+      repeat break_match; try solve_by_inversion.
+      +++ repeat find_inversion.
+          simpl in *.
+          repeat find_inversion.
+          edestruct IHt1; try reflexivity.
+          rewrite Heqp2.
+          simpl.
+          dunit.
+          eassumption.
+          econstructor.
+          rewrite Heqp2.
+          eassumption.
+          simpl.
+          econstructor.
+          simpl.
+          rewrite Heqp2.
+          Lemma allMappedL : forall r t1 t2 p st,
+            allMapped (alseq r t1 t2) p st ->
+            allMapped t1 p st.
+          Proof.
+          Admitted.
+
+          eapply allMappedL; eauto.
+          exists x.
+          dunit.
+          destruct_conjs.
+          unfold exec_app_comp_t in *.
+          unfold exec_app_comp in *.
+          monad_unfold.
+          unfold runSt in *.
+          rewrite Heqp2 in *.
+          simpl in *.
+          repeat break_match; try solve_by_inversion.
+          simpl in *.
+          repeat find_inversion.
+          destruct o; try solve_by_inversion.
+          repeat find_inversion.
+          admit.
+    ++
+      admit.
+    +
+      repeat break_let; simpl in *.
+      repeat find_inversion.
+      admit.
+  -
+    
+      
+      
+      +++ repeat find_inversion.
+          simpl in *.
+          
+          unfold gen_appraisal_comp in *
+    
+    invc H0.
+    
+      
+      
+      
+      
+      
+
+
+
+
+
+
+
+
+
+
+
+
+
+
+
+
+
+
+    
+    unfold allMapped.
+    intros; subst.
+      
+    unfold anno in Heqp1
+    cbn in H3.
+    break_let.
+    simpl in H3.
+    inv H3.
+    inv H2.
+    cbn in H.
+    break_let.
+    simpl in H.
+    clear H2.
+    clear H0.
+    
+
+    Check measEventAt'.
+    unfold annotated.
+    Check measEventAt'.
+    cbn in H4.
+    break_let.
+    simpl in H4.
+    eapply measEventAt'.
+    cbn.
+    break_let.
+    eassumption.
+
+    
+    cbn in H4.
+    repeat break_let.
+    simpl in H4.
+    simpl.
+    
+    repeat find_inversion.
+    unfold allMapped in H4.
+    inv H0.
+    edestruct H4.
+    apply H3.
+    reflexivity.
+
+    unfold allMapped.
+    intros.
+    subst.
+    cbn in H3.
+    break_let.
+    simpl in H3.
+
+    exists x.
+    
+    admit.
+    inv H1
+    apply H1.
+    eassumption.
+    intros.
+    subst.
+    
+
+    
+
+    
+
+
+
+    eapply measEventAt.
+    eassumption.
+    destruct_conjs.
+    monad_unfold.
+    unfold exec_app_comp_t.
+    unfold exec_app_comp.
+    monad_unfold.
+    unfold runSt.
+    break_match.
+    destruct o.
+    +
+      simpl.
+      destruct ast.
+      monad_unfold.
+      unfold runSt in *.
+      unfold exec_app_comp_t in *.
+      unfold exec_app_comp in *.
+      monad_unfold.
+      cbn in *.
+      repeat break_let.
+      simpl in *.
+      unfold build_app_comp in Heqp.
+      monad_unfold.
+      unfold run_vm_fresh in Heqp.
+      monad_unfold.
+      unfold run_vm in Heqp.
+      monad_unfold.
+      monad_unfold.
+      repeat break_let.
+      repeat find_inversion.
+      simpl in *.
+
+      Require Import MonadVMFacts.
+      vmsts.
+      simpl in *.
+      unfold get_store_at in *.
+      monad_unfold.
+      repeat break_let.
+      dohtac.
+      repeat find_inversion.
+      repeat break_match;
+        repeat find_inversion.
+      ++  vmsts.
+          vmsts.
+          inv H2.
+          unfold build_app_comp in *.
+          monad_unfold.
+          unfold run_vm_fresh in Heqp0.
+          unfold run_vm in *.
+          monad_unfold.
+          Print unanno.
+
+
+
+          rewrite announ in *.
+
+          Print build_comp.
+          repeat break_match;
+            try solve_by_inversion.
+          repeat find_inversion.
+
+          unfold runSt in *.
+
+
+
+          exists (umeas m q i' (args ++ [n0])).
+          split.
+
+          eapply atgentrace.
+          apply Heqp2.
+          apply Heqp1.
+          eassumption.
+          eauto.
+      ++
+        unfold build_app_comp in *.
+        monad_unfold.
+        repeat break_match;
+          try solve_by_inversion.
+    +
+      inv H3.
+      inv H2.
+      simpl.
+      unfold allMapped in *.
+      edestruct H4 with (st:=ast).
+      eassumption.
+      reflexivity.
+      repeat find_inversion.
+      unfold runSt in *.
+      monad_unfold.
+      unfold exec_app_comp_t in *.
+      unfold exec_app_comp in *.
+      monad_unfold.
+      repeat break_match;
+        try solve_by_inversion.
+      simpl in *.
+      unfold build_app_comp in *.
+      monad_unfold.
+      repeat break_match;
+        try solve_by_inversion.
+      ++ rewrite announ in *.
+         repeat find_inversion.
+         unfold run_vm_fresh in *.
+         unfold run_vm in *.
+         monad_unfold.
+         destruct ast.
+         simpl in *.
+
+
+
+         exfalso.
+         eapply fifi; eauto.
+      
+             
+  - 
+    
+          
+          
+              
+              
+   (*           
+              
+              unfold annotated in *.
+              rewrite <- IHt.
+              unfold anno in Heqp
+              
+              simpl.
+              
+            intros.
+            unfold annotated.
+            induction 
+            -
+              unfold anno. simpl. reflexivity.
+            - simpl. repeat break_let. simpl. unfold unanno
+              
+          Admitted.
+          
+
+            
+          unfold gen_appraisal_comp in *
+          inv H.
+          invc H7.
+          invc H7.
+          invc H8.
+          +++
+            unfold runSt in H1.
+            unfold build_app_comp in *.
+            monad_unfold.
+
+            destruct v.
+              simpl. vmsts.
+              simpl.
+              unfold gen_appraisal_comp in Heqp2.
+
+            
+          unfold gen_appraisal_comp in Heqp2
+    
+    
+      
+           
+ 
+         unfold bind.
+         unfold run_vm_fresh.
+         unfold run_vm.
+         unfold execSt.
+         unfold eval.
+         unfold annotated.
+         unfold anno.
+         simpl.
+         unfold bind.
+         unfold am_get_app_asp.
+         unfold bind.
+         unfold gets.
+         unfold bind.
+         unfold runSt.
+         unfold get.
+         repeat break_let.
+         repeat find_inversion.
+         repeat break_match.
+                     
+         monad_unfold.
+         unfold build_app_comp.
+         monad_unfold.
+         monad_unfold.
+         unfold am_get_app_asp.
+         monad_unfold.
+         repeat break_let.
+         unfold map_get
+         
+
+
+
+
+
+
+
+
+
+
+
+
+
+
+      
+      unfold runSt.
+      simpl in *.
+      repeat break_let.
+      simpl in *.
+      inv H1.
+      rewrite H2 in *.
+      invc Heqp0.
+      invc Heqp.
+      simpl.
+      eexists.
+      split.
+      right. left. eauto.
+      destruct a.
+      econstructor.
+      simpl in *.
+      assumption.
+    + invc H7.
+      invc H.
+      invc H0.
+    + invc H7.
+      invc H.
+      invc H0.
+  -
+    inv H7.
+    Print measEvent.
+    inv H0.
+    monad_unfold.
+    destruct empty_vmst.
+    simpl in *.
+    monad_unfold.
+    unfold runSt.
+    monad_unfold.
+
+    edestruct IHaterm0; eauto.
+    econstructor.
+    Lemma hfhf : forall x n t p,
+      ev_in x (ev_sys (annotated (att n t)) p) ->
+      ev_in x (ev_sys (annotated t) p).
+    Proof.
+    Admitted.
+    eapply hfhf; eauto.
+    econstructor.
+
+    (*
+    Lemma jfjf : forall n p t st,
+      allMapped (annotated (att n t)) p st ->
+      allMapped (annotated t) p st.
+    Proof.
+    Admitted.
+
+    eapply jfjf; eauto. *)
+    destruct_conjs.
+    inv H2.
+
+    exists (umeas m q i' (args ++ [n0])).
+    split.
+    unfold runSt in *.
+
+    Lemma jhjh : forall x t p n t_st init_st init_st',
+       In x
+         (StVM.st_trace
+            (snd
+               (build_comp
+                  (annotated
+                     (fromOpt
+                        (fst
+                           (gen_appraisal_term
+                              (StVM.st_ev
+                                 (run_vm (annotated t)
+                                    t_st))
+                              (eval t p mt)
+                              init_st)) 
+                        (asp CPY)))
+                  init_st'))) ->
+       In x
+         (StVM.st_trace
+            (snd
+               (build_comp
+                  (annotated
+                     (fromOpt
+                        (fst
+                           (gen_appraisal_term
+                              (StVM.st_ev
+                                 (run_vm (annotated (att n t))
+                                    t_st))
+                              (eval t n mt)
+                              init_st)) 
+                        (asp CPY)))
+                  init_st'))).
+    Proof.
+    Admitted.
+
+    eapply jhjh; eauto.
+    eauto.
+  - inv H7.
+    inv H0.
+    edestruct IHaterm0_1; eauto.
+    admit.
+
+*)
+  
+  
+  
+
