src/extra/Appraisal2.v
@@ -1,0 +1,363 @@
+Require Import GenStMonad MonadVM MonadAM ConcreteEvidence.
+Require Import StAM VM_IO_Axioms Maps VmSemantics Event_system Term_system.
+
+Require Import Coq.Arith.Peano_dec.
+
+
+Require Import List.
+Import ListNotations.
+
+Check map_get.
+
+Inductive evidenceEvent: Ev -> Prop :=
+| uev: forall n p i args, evidenceEvent (umeas n p i args)
+(*| sev: forall n p, evidenceEvent (sign n p)
+| hev: forall n p, evidenceEvent (hash n p)*) .
+
+Definition ioEvent (t:AnnoTerm) (p:Plc) (ev:Ev) : Prop :=
+  let es := ev_sys t p in
+  ev_in ev es /\ evidenceEvent ev.
+
+Check bound_to.
+
+Inductive appEvent : Ev -> AM_St -> Ev -> Prop :=
+| aeu : forall p q i i' n m args nmap nid amap,
+    bound_to amap (p,i) i' ->
+    appEvent (umeas n p i args) (mkAM_St nmap nid amap) (umeas m q i' (args ++ [n])).
+
+Definition am_get_app_asp (p:Plc) (i:ASP_ID) : AM ASP_ID :=
+  m <- gets st_aspmap ;;
+  let maybeId := map_get m (p,i) in
+  match maybeId with
+  | Some i' => ret i'
+  | None => failm
+  end.
+
+Fixpoint gen_appraisal_term (e:EvidenceC) (et:Evidence) : AM Term :=
+  match e with
+  | mtc =>
+    match et with
+    | mt => ret (asp CPY)
+    | _ => failm
+    end
+  | uuc i bs e' =>
+    match et with 
+    | uu i_t args_t p e'_t =>
+      app_id <- am_get_app_asp p i_t ;;
+      t2 <- gen_appraisal_term e' e'_t ;;
+      let t1 := (asp (ASPC app_id (args_t ++ [bs]))) in
+      let res := (bseq (NONE,NONE) t1 t2) in
+                     ret res
+    | _ => failm
+    end
+  | ssc e1 e2 =>
+    match et with
+    | ss e1_t e2_t => 
+      t1' <- (gen_appraisal_term e1 e1_t) ;;
+          t2' <- (gen_appraisal_term e2 e2_t) ;;
+          let res := (bseq (NONE,NONE) t1' t2') in (* BRP (NONE,NONE) t1' t2' *)
+          ret res
+    | _ => failm
+    end
+  | _ => ret (asp CPY)
+  end.
+    
+      (*
+  | ggc bs e' =>
+    match et with
+    | gg p e'_t =>
+        let sig_id := 42 in      (* sig_id <- am_get_sig_asp p *)
+        (* let evBits = encodeEv e' --BL.toStrict (DA.encode e)
+            evBitsArg = show evBits
+            sigArg = show bs *)
+        t2 <- gen_appraisal_term e' e'_t ;;
+        let t1 := (asp (ASPC sig_id)) in   (* (ASP sig_id [evBitsArg,sigArg]) *)
+        let res := (bpar (NONE,NONE) t1 t2) in   (* BRP (NONE,NONE) t1 t2 *)
+        ret res
+    | _ => failm
+    end
+  | hhc bs e' =>
+    match et with
+    | hh p e'_t =>
+        let hsh_id := 0 in      (* hsh_id <- am_get_hsh_asp p *)
+        (* let evBits = encodeEv e' --BL.toStrict (DA.encode e)
+            evBitsArg = show evBits
+            sigArg = show bs *)
+        t2 <- gen_appraisal_term e' e'_t ;;
+        let t1 := (asp (ASPC hsh_id)) in   (* (ASP sig_id [evBitsArg,sigArg]) *)
+        let res := (bpar (NONE,NONE) t1 t2) in   (* BRP (NONE,NONE) t1 t2 *)
+        ret res
+    | _ => failm
+    end
+  | ssc e1 e2 =>
+    match et with
+    | ss e1_t e2_t => 
+      t1' <- (gen_appraisal_term e1 e1_t) ;;
+          t2' <- (gen_appraisal_term e2 e2_t) ;;
+          let res := (bpar (NONE,NONE) t1' t2') in (* BRP (NONE,NONE) t1' t2' *)
+          ret res
+    | _ => failm
+    end
+  | ppc e1 e2 =>
+    match et with
+    | pp e1_t e2_t => 
+      t1' <- (gen_appraisal_term e1 e1_t) ;;
+          t2' <- (gen_appraisal_term e2 e2_t) ;;
+          let res := (bpar (NONE,NONE) t1' t2') in (* BRP (NONE,NONE) t1' t2' *)
+          ret res
+    | _ => failm
+    end      
+  | nnc _ _ _ =>  ret (asp CPY) (* Dummy nonce case for now.  TODO: robustify *)
+       
+  | _ => ret (asp CPY)
+end.
+*)
+
+Definition at1 := (asp (ASPC 1 [])).
+Definition at2 := (asp (ASPC 2 [])).
+Definition aterm := bseq (NONE,NONE) at1 at2.
+
+Definition aet := eval aterm 0 mt.
+Print aet.
+Compute aet.
+
+Definition evc_st := (run_vm (annotated aterm) empty_vmst).
+Compute evc_st.
+Definition evc := st_ev evc_st.
+Compute evc.
+
+Definition acomp := (gen_appraisal_term evc aet).
+Compute acomp.
+
+Check runSt.
+
+Definition ast :=
+  mkAM_St [] 0 [((0,1),33); ((0,2),44)].
+
+Definition appterm := (runSt ast acomp).
+Compute appterm.
+
+
+(*
+     = (Some
+          (bpar (NONE, NONE) (bpar (NONE, NONE) (asp (ASPC 3 [])) (asp CPY))
+             (bpar (NONE, NONE) (asp (ASPC 4 [])) (asp CPY))),
+       {| am_nonceMap := []; am_nonceId := 0; st_aspmap := [(0, 1, 3); (0, 2, 4)] |})
+     : option Term * AM_St
+*)
+
+Compute aet.
+(*
+     = ss (uu 1 0 mt) (uu 2 0 mt)
+     : Evidence
+ *)
+Definition evc_res := (run_vm (annotated aterm) empty_vmst).
+Compute evc.
+
+Definition fromOpt{A:Type} (o:option A) (a:A) : A :=
+  match o with
+  | Some t => t
+  | None => a
+  end.
+
+Definition app_term := fromOpt (fst appterm) (asp CPY).
+Compute app_term.
+
+(*
+
+Definition app_term' :=
+  (bpar (NONE, NONE) (asp (ASPC 44 [])) (asp CPY)).
+
+Definition app_term'' :=
+  (bpar (NONE, NONE) (asp (ASPC 33 [])) (asp (ASPC 44 [])) ).
+*)
+
+
+Definition app_comp := (build_comp (annotated (app_term))).
+
+Definition app_comp_res := runSt empty_vmst app_comp.
+Compute app_comp_res.
+Definition tr_app_comp := st_trace (snd app_comp_res).
+Compute tr_app_comp.
+
+Check In.
+
+Require Import StructTactics.
+
+Definition allMapped (t:AnnoTerm) (p:Plc) (st: AM_St) : Prop :=
+  forall t st aspmap n q i l ,
+    ioEvent t p (umeas n q i l) ->
+    aspmap = st_aspmap st ->
+    exists j,
+      bound_to aspmap (q,i) j.
+
+Set Nested Proofs Allowed.
+Require Import Coq.Program.Tactics Coq.Program.Equality.
+Lemma app_correct :
+  forall aterm ev ast aet evc acomp appterm app_term
+    app_comp app_comp_res tr_app_comp ,
+  aet = eval aterm 0 mt ->
+  evc = st_ev (run_vm (annotated aterm) empty_vmst) ->
+  acomp = (gen_appraisal_term evc aet) ->
+  appterm = (runSt ast acomp) ->
+  app_term = fromOpt (fst appterm) (asp CPY) ->
+  app_comp = (build_comp (annotated app_term)) ->
+  app_comp_res = runSt empty_vmst app_comp ->
+  tr_app_comp = st_trace (snd app_comp_res) ->
+                       
+  ioEvent (annotated aterm) 0 ev ->
+  allMapped (annotated aterm) 0 ast ->
+  exists ev', In ev' tr_app_comp /\ appEvent ev ast ev'.
+Proof.
+  induction aterm0; intros; subst.
+  -
+    destruct a.
+    +
+      invc H7.
+      invc H.
+      invc H0.
+    +
+      inv H7.
+      inv H.
+      repeat find_inversion.
+     
+      simpl.
+      monad_unfold.
+      unfold allMapped in *.
+      edestruct H8 with (st:=ast0).
+      apply H7.
+      reflexivity.
+      unfold am_get_app_asp.
+      monad_unfold.
+      simpl.
+      unfold runSt.
+      simpl in *.
+      repeat break_let.
+      simpl in *.
+      inv H1.
+      rewrite H2 in *.
+      invc Heqp0.
+      invc Heqp.
+      simpl.
+      eexists.
+      split.
+      right. left. eauto.
+      destruct a.
+      econstructor.
+      simpl in *.
+      assumption.
+    + invc H7.
+      invc H.
+      invc H0.
+    + invc H7.
+      invc H.
+      invc H0.
+  -
+    inv H7.
+    Print ioEvent.
+    inv H0.
+    monad_unfold.
+    destruct empty_vmst.
+    simpl in *.
+    monad_unfold.
+    unfold runSt.
+    monad_unfold.
+
+    edestruct IHaterm0; eauto.
+    econstructor.
+    Lemma hfhf : forall x n t p,
+      ev_in x (ev_sys (annotated (att n t)) p) ->
+      ev_in x (ev_sys (annotated t) p).
+    Proof.
+    Admitted.
+    eapply hfhf; eauto.
+    econstructor.
+
+    (*
+    Lemma jfjf : forall n p t st,
+      allMapped (annotated (att n t)) p st ->
+      allMapped (annotated t) p st.
+    Proof.
+    Admitted.
+
+    eapply jfjf; eauto. *)
+    destruct_conjs.
+    inv H2.
+
+    exists (umeas m q i' (args ++ [n0])).
+    split.
+    unfold runSt in *.
+
+    Lemma jhjh : forall x t p n t_st init_st init_st',
+       In x
+         (StVM.st_trace
+            (snd
+               (build_comp
+                  (annotated
+                     (fromOpt
+                        (fst
+                           (gen_appraisal_term
+                              (StVM.st_ev
+                                 (run_vm (annotated t)
+                                    t_st))
+                              (eval t p mt)
+                              init_st)) 
+                        (asp CPY)))
+                  init_st'))) ->
+       In x
+         (StVM.st_trace
+            (snd
+               (build_comp
+                  (annotated
+                     (fromOpt
+                        (fst
+                           (gen_appraisal_term
+                              (StVM.st_ev
+                                 (run_vm (annotated (att n t))
+                                    t_st))
+                              (eval t n mt)
+                              init_st)) 
+                        (asp CPY)))
+                  init_st'))).
+    Proof.
+    Admitted.
+
+    eapply jhjh; eauto.
+    eauto.
+  - inv H7.
+    inv H0.
+    edestruct IHaterm0_1; eauto.
+    admit.
+
+Lemma app_correct : forall ev,
+    ioEvent (annotated aterm) 0 ev ->
+    exists ev', In ev' tr_app_comp /\
+           appEvent ev ast ev'.
+Proof.
+  intros.
+  cbv in *.
+  invc H.
+  invc H0.
+  invc H3.
+  inv H1.
+  invc H3.
+  invc H2.
+  invc H3.
+  invc H1.
+  eexists.
+  split.
+  right. right. left. eauto.
+  econstructor.
+  econstructor. simpl. tauto.
+  invc H3. invc H1.
+  eexists.
+  split.
+  right. right. right. right. right. right. left. eauto.
+  econstructor.
+  econstructor. simpl. tauto.
+  invc H2. invc H1.
+Defined.
+  
+  
+  
+
